converting more HOL-Auth to new-style theories

src/HOL/Auth/Kerberos_BAN.thy
@@ -8,17 +8,23 @@ The Kerberos protocol, BAN version.
 From page 251 of
   Burrows, Abadi and Needham.  A Logic of Authentication.
   Proc. Royal Soc. 426 (1989)
+
+  Confidentiality (secrecy) and authentication properties rely on 
+  temporal checks: strong guarantees in a little abstracted - but
+  very realistic - model (see .thy).
+
+Tidied and converted to Isar by lcp.
 *)
 
-Kerberos_BAN = Shared + 
+theory Kerberos_BAN = Shared:
 
 (* Temporal modelization: session keys can be leaked 
                           ONLY when they have expired *)
 
 syntax
-    CT :: event list=>nat
-    Expired :: [nat, event list] => bool
-    RecentAuth :: [nat, event list] => bool
+    CT :: "event list=>nat"
+    Expired :: "[nat, event list] => bool"
+    RecentAuth :: "[nat, event list] => bool"
 
 consts
 
@@ -28,12 +34,12 @@ consts
     (*Duration of the authenticator*)
     AutLife :: nat
 
-rules
+axioms
     (*The ticket should remain fresh for two journeys on the network at least*)
-    SesKeyLife_LB "2 <= SesKeyLife"
+    SesKeyLife_LB: "2 <= SesKeyLife"
 
     (*The authenticator only for one journey*)
-    AutLife_LB    "Suc 0 <= AutLife"
+    AutLife_LB:    "Suc 0 <= AutLife"
 
 translations
    "CT" == "length"
@@ -42,51 +48,382 @@ translations
 
    "RecentAuth T evs" == "CT evs <= AutLife + T"
 
-consts  kerberos_ban   :: event list set
+consts  kerberos_ban   :: "event list set"
 inductive "kerberos_ban"
-  intrs 
+ intros 
 
-    Nil  "[] \\<in> kerberos_ban"
+   Nil:  "[] \<in> kerberos_ban"
 
-    Fake "[| evsf \\<in> kerberos_ban;  X \\<in> synth (analz (spies evsf)) |]
-          ==> Says Spy B X # evsf \\<in> kerberos_ban"
-
-
-    Kb1  "[| evs1 \\<in> kerberos_ban |]
-          ==> Says A Server {|Agent A, Agent B|} # evs1
-                \\<in>  kerberos_ban"
+   Fake: "[| evsf \<in> kerberos_ban;  X \<in> synth (analz (spies evsf)) |]
+	  ==> Says Spy B X # evsf \<in> kerberos_ban"
 
 
-    Kb2  "[| evs2 \\<in> kerberos_ban;  Key KAB \\<notin> used evs2;
-             Says A' Server {|Agent A, Agent B|} \\<in> set evs2 |]
-          ==> Says Server A 
-                (Crypt (shrK A)
-                   {|Number (CT evs2), Agent B, Key KAB,  
-                    (Crypt (shrK B) {|Number (CT evs2), Agent A, Key KAB|})|}) 
-                # evs2 \\<in> kerberos_ban"
+   Kb1:  "[| evs1 \<in> kerberos_ban |]
+	  ==> Says A Server {|Agent A, Agent B|} # evs1
+		\<in>  kerberos_ban"
 
 
-    Kb3  "[| evs3 \\<in> kerberos_ban;  
-             Says S A (Crypt (shrK A) {|Number Ts, Agent B, Key K, X|}) 
-               \\<in> set evs3;
-             Says A Server {|Agent A, Agent B|} \\<in> set evs3;
-             ~ Expired Ts evs3 |]
-          ==> Says A B {|X, Crypt K {|Agent A, Number (CT evs3)|} |} 
-               # evs3 \\<in> kerberos_ban"
+   Kb2:  "[| evs2 \<in> kerberos_ban;  Key KAB \<notin> used evs2;
+	     Says A' Server {|Agent A, Agent B|} \<in> set evs2 |]
+	  ==> Says Server A 
+		(Crypt (shrK A)
+		   {|Number (CT evs2), Agent B, Key KAB,  
+		    (Crypt (shrK B) {|Number (CT evs2), Agent A, Key KAB|})|}) 
+		# evs2 \<in> kerberos_ban"
 
 
-    Kb4  "[| evs4 \\<in> kerberos_ban;  
-             Says A' B {|(Crypt (shrK B) {|Number Ts, Agent A, Key K|}), 
-		         (Crypt K {|Agent A, Number Ta|}) |}: set evs4;
-             ~ Expired Ts evs4;  RecentAuth Ta evs4 |]
-          ==> Says B A (Crypt K (Number Ta)) # evs4
-                \\<in> kerberos_ban"
+   Kb3:  "[| evs3 \<in> kerberos_ban;  
+	     Says S A (Crypt (shrK A) {|Number Ts, Agent B, Key K, X|}) 
+	       \<in> set evs3;
+	     Says A Server {|Agent A, Agent B|} \<in> set evs3;
+	     ~ Expired Ts evs3 |]
+	  ==> Says A B {|X, Crypt K {|Agent A, Number (CT evs3)|} |} 
+	       # evs3 \<in> kerberos_ban"
 
-         (*Old session keys may become compromised*)
-    Oops "[| evso \\<in> kerberos_ban;  
-             Says Server A (Crypt (shrK A) {|Number Ts, Agent B, Key K, X|})
-               \\<in> set evso;
-             Expired Ts evso |]
-          ==> Notes Spy {|Number Ts, Key K|} # evso \\<in> kerberos_ban"
+
+   Kb4:  "[| evs4 \<in> kerberos_ban;  
+	     Says A' B {|(Crypt (shrK B) {|Number Ts, Agent A, Key K|}), 
+			 (Crypt K {|Agent A, Number Ta|}) |}: set evs4;
+	     ~ Expired Ts evs4;  RecentAuth Ta evs4 |]
+	  ==> Says B A (Crypt K (Number Ta)) # evs4
+		\<in> kerberos_ban"
+
+	(*Old session keys may become compromised*)
+   Oops: "[| evso \<in> kerberos_ban;  
+	     Says Server A (Crypt (shrK A) {|Number Ts, Agent B, Key K, X|})
+	       \<in> set evso;
+	     Expired Ts evso |]
+	  ==> Notes Spy {|Number Ts, Key K|} # evso \<in> kerberos_ban"
+
+
+declare Says_imp_knows_Spy [THEN parts.Inj, dest] parts.Body [dest]
+declare analz_subset_parts [THEN subsetD, dest]
+declare Fake_parts_insert [THEN subsetD, dest]
+
+declare SesKeyLife_LB [iff] AutLife_LB [iff]
+
+
+(*A "possibility property": there are traces that reach the end.*)
+lemma "\<exists>Timestamp K. \<exists>evs \<in> kerberos_ban.     
+             Says B A (Crypt K (Number Timestamp))  
+                  \<in> set evs"
+apply (cut_tac SesKeyLife_LB)
+apply (intro exI bexI)
+apply (rule_tac [2] 
+           kerberos_ban.Nil [THEN kerberos_ban.Kb1, THEN kerberos_ban.Kb2, 
+                             THEN kerberos_ban.Kb3, THEN kerberos_ban.Kb4], possibility)
+apply (simp_all (no_asm_simp))
+done
+
+
+(**** Inductive proofs about kerberos_ban ****)
+
+(*Forwarding Lemma for reasoning about the encrypted portion of message Kb3*)
+lemma Kb3_msg_in_parts_spies:
+     "Says S A (Crypt KA {|Timestamp, B, K, X|}) \<in> set evs  
+      ==> X \<in> parts (spies evs)"
+by blast
+                              
+lemma Oops_parts_spies:
+     "Says Server A (Crypt (shrK A) {|Timestamp, B, K, X|}) \<in> set evs  
+      ==> K \<in> parts (spies evs)"
+by blast
+
+
+(*Spy never sees another agent's shared key! (unless it's bad at start)*)
+lemma Spy_see_shrK [simp]:
+     "evs \<in> kerberos_ban ==> (Key (shrK A) \<in> parts (spies evs)) = (A \<in> bad)"
+apply (erule kerberos_ban.induct) 
+apply (frule_tac [7] Oops_parts_spies) 
+apply (frule_tac [5] Kb3_msg_in_parts_spies, simp_all)  
+apply blast+
+done
+
+
+lemma Spy_analz_shrK [simp]:
+     "evs \<in> kerberos_ban ==> (Key (shrK A) \<in> analz (spies evs)) = (A \<in> bad)"
+apply auto
+done
+
+
+lemma Spy_see_shrK_D [dest!]:
+     "[| Key (shrK A) \<in> parts (spies evs);        
+                evs \<in> kerberos_ban |] ==> A:bad"
+apply (blast dest: Spy_see_shrK)
+done
+
+lemmas Spy_analz_shrK_D = analz_subset_parts [THEN subsetD, THEN Spy_see_shrK_D,  dest!]
+
+
+(*Nobody can have used non-existent keys!*)
+lemma new_keys_not_used [rule_format, simp]:
+     "evs \<in> kerberos_ban ==>       
+       Key K \<notin> used evs --> K \<notin> keysFor (parts (spies evs))"
+apply (erule kerberos_ban.induct) 
+apply (frule_tac [7] Oops_parts_spies) 
+apply (frule_tac [5] Kb3_msg_in_parts_spies, simp_all)  
+(*Fake*)
+apply (force dest!: keysFor_parts_insert)
+(*Kb2, Kb3, Kb4*)
+apply blast+
+done
+
+(** Lemmas concerning the form of items passed in messages **)
+
+(*Describes the form of K, X and K' when the Server sends this message.*)
+lemma Says_Server_message_form:
+     "[| Says Server A (Crypt K' {|Number Ts, Agent B, Key K, X|})   
+         \<in> set evs; evs \<in> kerberos_ban |]                            
+      ==> K \<notin> range shrK &                                          
+          X = (Crypt (shrK B) {|Number Ts, Agent A, Key K|}) &       
+          K' = shrK A"
+apply (erule rev_mp)
+apply (erule kerberos_ban.induct, auto)
+done
+
+
+(*If the encrypted message appears then it originated with the Server
+  PROVIDED that A is NOT compromised!
+
+  This shows implicitly the FRESHNESS OF THE SESSION KEY to A
+*)
+lemma A_trusts_K_by_Kb2:
+     "[| Crypt (shrK A) {|Number Ts, Agent B, Key K, X|}  
+           \<in> parts (spies evs);                           
+         A \<notin> bad;  evs \<in> kerberos_ban |]                 
+       ==> Says Server A (Crypt (shrK A) {|Number Ts, Agent B, Key K, X|})  
+             \<in> set evs"
+apply (erule rev_mp)
+apply (erule kerberos_ban.induct) 
+apply (frule_tac [7] Oops_parts_spies) 
+apply (frule_tac [5] Kb3_msg_in_parts_spies, simp_all)  
+apply blast
+done
+
+
+(*If the TICKET appears then it originated with the Server*)
+(*FRESHNESS OF THE SESSION KEY to B*)
+lemma B_trusts_K_by_Kb3:
+     "[| Crypt (shrK B) {|Number Ts, Agent A, Key K|} \<in> parts (spies evs);  
+         B \<notin> bad;  evs \<in> kerberos_ban |]                         
+       ==> Says Server A                                          
+            (Crypt (shrK A) {|Number Ts, Agent B, Key K,                    
+                          Crypt (shrK B) {|Number Ts, Agent A, Key K|}|})   
+           \<in> set evs"
+apply (erule rev_mp)
+apply (erule kerberos_ban.induct) 
+apply (frule_tac [7] Oops_parts_spies) 
+apply (frule_tac [5] Kb3_msg_in_parts_spies, simp_all)  
+apply blast
+done
+
+
+(*EITHER describes the form of X when the following message is sent, 
+  OR     reduces it to the Fake case.
+  Use Says_Server_message_form if applicable.*)
+lemma Says_S_message_form:
+     "[| Says S A (Crypt (shrK A) {|Number Ts, Agent B, Key K, X|})      
+            \<in> set evs;                                                   
+         evs \<in> kerberos_ban |]                                           
+ ==> (K \<notin> range shrK & X = (Crypt (shrK B) {|Number Ts, Agent A, Key K|})) 
+          | X \<in> analz (spies evs)"
+apply (case_tac "A \<in> bad")
+apply (force dest!: Says_imp_spies [THEN analz.Inj])
+apply (frule Says_imp_spies [THEN parts.Inj])
+apply (blast dest!: A_trusts_K_by_Kb2 Says_Server_message_form)
+done
+
+
+
+(****
+ The following is to prove theorems of the form
+
+  Key K \<in> analz (insert (Key KAB) (spies evs)) ==>
+  Key K \<in> analz (spies evs)
+
+ A more general formula must be proved inductively.
+
+****)
+
+
+(** Session keys are not used to encrypt other session keys **)
+
+lemma analz_image_freshK [rule_format (no_asm)]:
+     "evs \<in> kerberos_ban ==>                           
+   \<forall>K KK. KK <= - (range shrK) -->                  
+          (Key K \<in> analz (Key`KK Un (spies evs))) =   
+          (K \<in> KK | Key K \<in> analz (spies evs))"
+apply (erule kerberos_ban.induct)
+apply (drule_tac [7] Says_Server_message_form)
+apply (erule_tac [5] Says_S_message_form [THEN disjE], analz_freshK, spy_analz)
+done
+
+
+
+lemma analz_insert_freshK:
+     "[| evs \<in> kerberos_ban;  KAB \<notin> range shrK |] ==>      
+      (Key K \<in> analz (insert (Key KAB) (spies evs))) =        
+      (K = KAB | Key K \<in> analz (spies evs))"
+by (simp only: analz_image_freshK analz_image_freshK_simps)
+
+
+(** The session key K uniquely identifies the message **)
+
+lemma unique_session_keys:
+     "[| Says Server A                                     
+           (Crypt (shrK A) {|Number Ts, Agent B, Key K, X|}) \<in> set evs;   
+         Says Server A'                                    
+          (Crypt (shrK A') {|Number Ts', Agent B', Key K, X'|}) \<in> set evs; 
+         evs \<in> kerberos_ban |] ==> A=A' & Ts=Ts' & B=B' & X = X'"
+apply (erule rev_mp)
+apply (erule rev_mp)
+apply (erule kerberos_ban.induct) 
+apply (frule_tac [7] Oops_parts_spies) 
+apply (frule_tac [5] Kb3_msg_in_parts_spies, simp_all)  
+(*Kb2: it can't be a new key*)
+apply blast
+done
+
+
+(** Lemma: the session key sent in msg Kb2 would be EXPIRED
+    if the spy could see it!
+**)
+
+lemma lemma2 [rule_format (no_asm)]:
+     "[| A \<notin> bad;  B \<notin> bad;  evs \<in> kerberos_ban |]            
+  ==> Says Server A                                             
+          (Crypt (shrK A) {|Number Ts, Agent B, Key K,          
+                            Crypt (shrK B) {|Number Ts, Agent A, Key K|}|}) 
+         \<in> set evs -->                                          
+      Key K \<in> analz (spies evs) --> Expired Ts evs"
+apply (erule kerberos_ban.induct)
+apply (frule_tac [7] Says_Server_message_form)
+apply (frule_tac [5] Says_S_message_form [THEN disjE])
+apply (simp_all (no_asm_simp) add: less_SucI analz_insert_eq analz_insert_freshK pushes)
+txt{*Fake*}
+apply spy_analz
+txt{*Kb2*}
+apply (blast intro: parts_insertI less_SucI)
+txt{*Kb3*}
+apply (case_tac "Aa \<in> bad")
+ prefer 2 apply (blast dest: A_trusts_K_by_Kb2 unique_session_keys)
+apply (blast dest: Says_imp_spies [THEN analz.Inj] Crypt_Spy_analz_bad elim!: MPair_analz intro: less_SucI)
+txt{*Oops: PROOF FAILED if addIs below*}
+apply (blast dest: unique_session_keys intro!: less_SucI)
+done
+
+
+(** CONFIDENTIALITY for the SERVER:
+                     Spy does not see the keys sent in msg Kb2 
+                     as long as they have NOT EXPIRED
+**)
+lemma Confidentiality_S:
+     "[| Says Server A                                            
+          (Crypt K' {|Number T, Agent B, Key K, X|}) \<in> set evs;   
+         ~ Expired T evs;                                         
+         A \<notin> bad;  B \<notin> bad;  evs \<in> kerberos_ban                 
+      |] ==> Key K \<notin> analz (spies evs)"
+apply (frule Says_Server_message_form, assumption)
+apply (blast intro: lemma2)
+done
+
+(**** THE COUNTERPART OF CONFIDENTIALITY 
+      [|...; Expired Ts evs; ...|] ==> Key K \<in> analz (spies evs)
+      WOULD HOLD ONLY IF AN OOPS OCCURRED! ---> Nothing to prove!   ****)
+
+
+(** CONFIDENTIALITY for ALICE: **)
+(** Also A_trusts_K_by_Kb2 RS Confidentiality_S **)
+lemma Confidentiality_A:
+     "[| Crypt (shrK A) {|Number T, Agent B, Key K, X|} \<in> parts (spies evs); 
+         ~ Expired T evs;           
+         A \<notin> bad;  B \<notin> bad;  evs \<in> kerberos_ban                 
+      |] ==> Key K \<notin> analz (spies evs)"
+apply (blast dest!: A_trusts_K_by_Kb2 Confidentiality_S)
+done
+
+
+(** CONFIDENTIALITY for BOB: **)
+(** Also B_trusts_K_by_Kb3 RS Confidentiality_S **)
+lemma Confidentiality_B:
+     "[| Crypt (shrK B) {|Number Tk, Agent A, Key K|}  
+          \<in> parts (spies evs);               
+        ~ Expired Tk evs;           
+        A \<notin> bad;  B \<notin> bad;  evs \<in> kerberos_ban                 
+      |] ==> Key K \<notin> analz (spies evs)"
+apply (blast dest!: B_trusts_K_by_Kb3 Confidentiality_S)
+done
+
+
+lemma lemma_B [rule_format]:
+     "[| B \<notin> bad;  evs \<in> kerberos_ban |]                         
+      ==> Key K \<notin> analz (spies evs) -->                     
+          Says Server A (Crypt (shrK A) {|Number Ts, Agent B, Key K, X|})  
+          \<in> set evs -->                                              
+          Crypt K (Number Ta) \<in> parts (spies evs) -->         
+          Says B A (Crypt K (Number Ta)) \<in> set evs"
+apply (erule kerberos_ban.induct)
+apply (frule_tac [7] Oops_parts_spies)
+apply (frule_tac [5] Says_S_message_form)
+apply (drule_tac [6] Kb3_msg_in_parts_spies, analz_mono_contra)
+apply (simp_all (no_asm_simp) add: all_conj_distrib)
+txt{*Fake*}
+apply blast
+txt{*Kb2*}
+apply (force dest: Crypt_imp_invKey_keysFor) 
+txt{*Kb4*}
+apply (blast dest: B_trusts_K_by_Kb3 unique_session_keys 
+                   Says_imp_spies [THEN analz.Inj] Crypt_Spy_analz_bad)
+done
+
+
+(*AUTHENTICATION OF B TO A*)
+lemma Authentication_B:
+     "[| Crypt K (Number Ta) \<in> parts (spies evs);            
+         Crypt (shrK A) {|Number Ts, Agent B, Key K, X|}     
+         \<in> parts (spies evs);                                
+         ~ Expired Ts evs;                                   
+         A \<notin> bad;  B \<notin> bad;  evs \<in> kerberos_ban |]         
+      ==> Says B A (Crypt K (Number Ta)) \<in> set evs"
+by (blast dest!: A_trusts_K_by_Kb2
+          intro!: lemma_B elim!: Confidentiality_S [THEN [2] rev_notE])
+
+
+
+lemma lemma_A [rule_format]:
+     "[| A \<notin> bad; B \<notin> bad; evs \<in> kerberos_ban |] 
+      ==>           
+         Key K \<notin> analz (spies evs) -->          
+         Says Server A (Crypt (shrK A) {|Number Ts, Agent B, Key K, X|})   
+         \<in> set evs -->   
+          Crypt K {|Agent A, Number Ta|} \<in> parts (spies evs) --> 
+         Says A B {|X, Crypt K {|Agent A, Number Ta|}|}   
+             \<in> set evs"
+apply (erule kerberos_ban.induct)
+apply (frule_tac [7] Oops_parts_spies)
+apply (frule_tac [5] Says_S_message_form)
+apply (frule_tac [6] Kb3_msg_in_parts_spies, analz_mono_contra)
+apply (simp_all (no_asm_simp) add: all_conj_distrib)
+txt{*Fake*}
+apply blast
+txt{*Kb2*}
+apply (force dest: Crypt_imp_invKey_keysFor) 
+txt{*Kb3*}
+apply (blast dest: A_trusts_K_by_Kb2 unique_session_keys)
+done
+
+
+(*AUTHENTICATION OF A TO B*)
+lemma Authentication_A:
+     "[| Crypt K {|Agent A, Number Ta|} \<in> parts (spies evs);   
+         Crypt (shrK B) {|Number Ts, Agent A, Key K|}          
+         \<in> parts (spies evs);                                  
+         ~ Expired Ts evs;                                     
+         A \<notin> bad;  B \<notin> bad;  evs \<in> kerberos_ban |]           
+      ==> Says A B {|Crypt (shrK B) {|Number Ts, Agent A, Key K|},      
+                     Crypt K {|Agent A, Number Ta|}|} \<in> set evs"
+by (blast dest!: B_trusts_K_by_Kb3
+          intro!: lemma_A 
+          elim!: Confidentiality_S [THEN [2] rev_notE])
 
 end
