src/HOL/Auth/NS_Shared.thy
@@ -16,60 +16,60 @@ consts  ns_shared   :: "event list set"
 inductive "ns_shared"
  intros
 	(*Initial trace is empty*)
-  Nil:  "[] \\<in> ns_shared"
+  Nil:  "[] \<in> ns_shared"
 	(*The spy MAY say anything he CAN say.  We do not expect him to
 	  invent new nonces here, but he can also use NS1.  Common to
 	  all similar protocols.*)
-  Fake: "\\<lbrakk>evsf \\<in> ns_shared;  X \\<in> synth (analz (spies evsf))\\<rbrakk>
-	 \\<Longrightarrow> Says Spy B X # evsf \\<in> ns_shared"
+  Fake: "\<lbrakk>evsf \<in> ns_shared;  X \<in> synth (analz (spies evsf))\<rbrakk>
+	 \<Longrightarrow> Says Spy B X # evsf \<in> ns_shared"
 
 	(*Alice initiates a protocol run, requesting to talk to any B*)
-  NS1:  "\\<lbrakk>evs1 \\<in> ns_shared;  Nonce NA \\<notin> used evs1\\<rbrakk>
-	 \\<Longrightarrow> Says A Server \\<lbrace>Agent A, Agent B, Nonce NA\\<rbrace> # evs1  \\<in>  ns_shared"
+  NS1:  "\<lbrakk>evs1 \<in> ns_shared;  Nonce NA \<notin> used evs1\<rbrakk>
+	 \<Longrightarrow> Says A Server \<lbrace>Agent A, Agent B, Nonce NA\<rbrace> # evs1  \<in>  ns_shared"
 
 	(*Server's response to Alice's message.
 	  !! It may respond more than once to A's request !!
 	  Server doesn't know who the true sender is, hence the A' in
 	      the sender field.*)
-  NS2:  "\\<lbrakk>evs2 \\<in> ns_shared;  Key KAB \\<notin> used evs2;
-	  Says A' Server \\<lbrace>Agent A, Agent B, Nonce NA\\<rbrace> \\<in> set evs2\\<rbrakk>
-	 \\<Longrightarrow> Says Server A
+  NS2:  "\<lbrakk>evs2 \<in> ns_shared;  Key KAB \<notin> used evs2;
+	  Says A' Server \<lbrace>Agent A, Agent B, Nonce NA\<rbrace> \<in> set evs2\<rbrakk>
+	 \<Longrightarrow> Says Server A
 	       (Crypt (shrK A)
-		  \\<lbrace>Nonce NA, Agent B, Key KAB,
-		    (Crypt (shrK B) \\<lbrace>Key KAB, Agent A\\<rbrace>)\\<rbrace>)
-	       # evs2 \\<in> ns_shared"
+		  \<lbrace>Nonce NA, Agent B, Key KAB,
+		    (Crypt (shrK B) \<lbrace>Key KAB, Agent A\<rbrace>)\<rbrace>)
+	       # evs2 \<in> ns_shared"
 
 	 (*We can't assume S=Server.  Agent A "remembers" her nonce.
-	   Need A \\<noteq> Server because we allow messages to self.*)
-  NS3:  "\\<lbrakk>evs3 \\<in> ns_shared;  A \\<noteq> Server;
-	  Says S A (Crypt (shrK A) \\<lbrace>Nonce NA, Agent B, Key K, X\\<rbrace>) \\<in> set evs3;
-	  Says A Server \\<lbrace>Agent A, Agent B, Nonce NA\\<rbrace> \\<in> set evs3\\<rbrakk>
-	 \\<Longrightarrow> Says A B X # evs3 \\<in> ns_shared"
+	   Need A \<noteq> Server because we allow messages to self.*)
+  NS3:  "\<lbrakk>evs3 \<in> ns_shared;  A \<noteq> Server;
+	  Says S A (Crypt (shrK A) \<lbrace>Nonce NA, Agent B, Key K, X\<rbrace>) \<in> set evs3;
+	  Says A Server \<lbrace>Agent A, Agent B, Nonce NA\<rbrace> \<in> set evs3\<rbrakk>
+	 \<Longrightarrow> Says A B X # evs3 \<in> ns_shared"
 
 	(*Bob's nonce exchange.  He does not know who the message came
 	  from, but responds to A because she is mentioned inside.*)
-  NS4:  "\\<lbrakk>evs4 \\<in> ns_shared;  Nonce NB \\<notin> used evs4;
-	  Says A' B (Crypt (shrK B) \\<lbrace>Key K, Agent A\\<rbrace>) \\<in> set evs4\\<rbrakk>
-	 \\<Longrightarrow> Says B A (Crypt K (Nonce NB)) # evs4 \\<in> ns_shared"
+  NS4:  "\<lbrakk>evs4 \<in> ns_shared;  Nonce NB \<notin> used evs4;
+	  Says A' B (Crypt (shrK B) \<lbrace>Key K, Agent A\<rbrace>) \<in> set evs4\<rbrakk>
+	 \<Longrightarrow> Says B A (Crypt K (Nonce NB)) # evs4 \<in> ns_shared"
 
 	(*Alice responds with Nonce NB if she has seen the key before.
 	  Maybe should somehow check Nonce NA again.
 	  We do NOT send NB-1 or similar as the Spy cannot spoof such things.
 	  Letting the Spy add or subtract 1 lets him send all nonces.
 	  Instead we distinguish the messages by sending the nonce twice.*)
-  NS5:  "\\<lbrakk>evs5 \\<in> ns_shared;
-	  Says B' A (Crypt K (Nonce NB)) \\<in> set evs5;
-	  Says S  A (Crypt (shrK A) \\<lbrace>Nonce NA, Agent B, Key K, X\\<rbrace>)
-	    \\<in> set evs5\\<rbrakk>
-	 \\<Longrightarrow> Says A B (Crypt K \\<lbrace>Nonce NB, Nonce NB\\<rbrace>) # evs5 \\<in> ns_shared"
+  NS5:  "\<lbrakk>evs5 \<in> ns_shared;
+	  Says B' A (Crypt K (Nonce NB)) \<in> set evs5;
+	  Says S  A (Crypt (shrK A) \<lbrace>Nonce NA, Agent B, Key K, X\<rbrace>)
+	    \<in> set evs5\<rbrakk>
+	 \<Longrightarrow> Says A B (Crypt K \<lbrace>Nonce NB, Nonce NB\<rbrace>) # evs5 \<in> ns_shared"
 
 	(*This message models possible leaks of session keys.
 	  The two Nonces identify the protocol run: the rule insists upon
 	  the true senders in order to make them accurate.*)
-  Oops: "\\<lbrakk>evso \\<in> ns_shared;  Says B A (Crypt K (Nonce NB)) \\<in> set evso;
-	  Says Server A (Crypt (shrK A) \\<lbrace>Nonce NA, Agent B, Key K, X\\<rbrace>)
-	      \\<in> set evso\\<rbrakk>
-	 \\<Longrightarrow> Notes Spy \\<lbrace>Nonce NA, Nonce NB, Key K\\<rbrace> # evso \\<in> ns_shared"
+  Oops: "\<lbrakk>evso \<in> ns_shared;  Says B A (Crypt K (Nonce NB)) \<in> set evso;
+	  Says Server A (Crypt (shrK A) \<lbrace>Nonce NA, Agent B, Key K, X\<rbrace>)
+	      \<in> set evso\<rbrakk>
+	 \<Longrightarrow> Notes Spy \<lbrace>Nonce NA, Nonce NB, Key K\<rbrace> # evso \<in> ns_shared"
 
 
 declare Says_imp_knows_Spy [THEN parts.Inj, dest]
@@ -79,9 +79,9 @@ declare analz_into_parts [dest]
 declare image_eq_UN [simp]  (*accelerates proofs involving nested images*)
 
 
-(*A "possibility property": there are traces that reach the end*)
-lemma "A \\<noteq> Server \\<Longrightarrow> \\<exists>N K. \\<exists>evs \\<in> ns_shared.
-                              Says A B (Crypt K \\<lbrace>Nonce N, Nonce N\\<rbrace>) \\<in> set evs"
+text{*A "possibility property": there are traces that reach the end*}
+lemma "A \<noteq> Server \<Longrightarrow> \<exists>N K. \<exists>evs \<in> ns_shared.
+                              Says A B (Crypt K \<lbrace>Nonce N, Nonce N\<rbrace>) \<in> set evs"
 apply (intro exI bexI)
 apply (rule_tac [2] ns_shared.Nil
        [THEN ns_shared.NS1, THEN ns_shared.NS2, THEN ns_shared.NS3,
@@ -89,94 +89,94 @@ apply (rule_tac [2] ns_shared.Nil
 done
 
 (*This version is similar, while instantiating ?K and ?N to epsilon-terms
-lemma "A \\<noteq> Server \\<Longrightarrow> \\<exists>evs \\<in> ns_shared.
-                Says A B (Crypt ?K \\<lbrace>Nonce ?N, Nonce ?N\\<rbrace>) \\<in> set evs"
+lemma "A \<noteq> Server \<Longrightarrow> \<exists>evs \<in> ns_shared.
+                Says A B (Crypt ?K \<lbrace>Nonce ?N, Nonce ?N\<rbrace>) \<in> set evs"
 *)
 
 
-(**** Inductive proofs about ns_shared ****)
+subsection{*Inductive proofs about @{term ns_shared}*}
 
-(** Forwarding lemmas, to aid simplification **)
+subsubsection{*Forwarding lemmas, to aid simplification*}
 
-(*For reasoning about the encrypted portion of message NS3*)
+text{*For reasoning about the encrypted portion of message NS3*}
 lemma NS3_msg_in_parts_spies:
-     "Says S A (Crypt KA \\<lbrace>N, B, K, X\\<rbrace>) \\<in> set evs \\<Longrightarrow> X \\<in> parts (spies evs)"
+     "Says S A (Crypt KA \<lbrace>N, B, K, X\<rbrace>) \<in> set evs \<Longrightarrow> X \<in> parts (spies evs)"
 by blast
 
-(*For reasoning about the Oops message*)
+text{*For reasoning about the Oops message*}
 lemma Oops_parts_spies:
-     "Says Server A (Crypt (shrK A) \\<lbrace>NA, B, K, X\\<rbrace>) \\<in> set evs
-            \\<Longrightarrow> K \\<in> parts (spies evs)"
+     "Says Server A (Crypt (shrK A) \<lbrace>NA, B, K, X\<rbrace>) \<in> set evs
+            \<Longrightarrow> K \<in> parts (spies evs)"
 by blast
 
-(** Theorems of the form X \\<notin> parts (spies evs) imply that NOBODY
-    sends messages containing X! **)
+text{*Theorems of the form @{term "X \<notin> parts (spies evs)"} imply that NOBODY
+    sends messages containing @{term X}*}
 
-(*Spy never sees another agent's shared key! (unless it's bad at start)*)
+text{*Spy never sees another agent's shared key! (unless it's bad at start)*}
 lemma Spy_see_shrK [simp]:
-     "evs \\<in> ns_shared \\<Longrightarrow> (Key (shrK A) \\<in> parts (spies evs)) = (A \\<in> bad)"
+     "evs \<in> ns_shared \<Longrightarrow> (Key (shrK A) \<in> parts (spies evs)) = (A \<in> bad)"
 apply (erule ns_shared.induct, force, drule_tac [4] NS3_msg_in_parts_spies, simp_all, blast+)
 done
 
 lemma Spy_analz_shrK [simp]:
-     "evs \\<in> ns_shared \\<Longrightarrow> (Key (shrK A) \\<in> analz (spies evs)) = (A \\<in> bad)"
+     "evs \<in> ns_shared \<Longrightarrow> (Key (shrK A) \<in> analz (spies evs)) = (A \<in> bad)"
 by auto
 
 
-(*Nobody can have used non-existent keys!*)
+text{*Nobody can have used non-existent keys!*}
 lemma new_keys_not_used [rule_format, simp]:
-    "evs \\<in> ns_shared \\<Longrightarrow> Key K \\<notin> used evs \\<longrightarrow> K \\<notin> keysFor (parts (spies evs))"
+    "evs \<in> ns_shared \<Longrightarrow> Key K \<notin> used evs \<longrightarrow> K \<notin> keysFor (parts (spies evs))"
 apply (erule ns_shared.induct, force, drule_tac [4] NS3_msg_in_parts_spies, simp_all)
-(*Fake, NS2, NS4, NS5*)
-apply (blast dest!: keysFor_parts_insert)+
+txt{*Fake, NS2, NS4, NS5*}
+apply (force dest!: keysFor_parts_insert, blast+)
 done
 
 
-(** Lemmas concerning the form of items passed in messages **)
+subsubsection{*Lemmas concerning the form of items passed in messages*}
 
-(*Describes the form of K, X and K' when the Server sends this message.*)
+text{*Describes the form of K, X and K' when the Server sends this message.*}
 lemma Says_Server_message_form:
-     "\\<lbrakk>Says Server A (Crypt K' \\<lbrace>N, Agent B, Key K, X\\<rbrace>) \\<in> set evs;
-       evs \\<in> ns_shared\\<rbrakk>
-      \\<Longrightarrow> K \\<notin> range shrK \\<and>
-          X = (Crypt (shrK B) \\<lbrace>Key K, Agent A\\<rbrace>) \\<and>
+     "\<lbrakk>Says Server A (Crypt K' \<lbrace>N, Agent B, Key K, X\<rbrace>) \<in> set evs;
+       evs \<in> ns_shared\<rbrakk>
+      \<Longrightarrow> K \<notin> range shrK \<and>
+          X = (Crypt (shrK B) \<lbrace>Key K, Agent A\<rbrace>) \<and>
           K' = shrK A"
 by (erule rev_mp, erule ns_shared.induct, auto)
 
 
-(*If the encrypted message appears then it originated with the Server*)
+text{*If the encrypted message appears then it originated with the Server*}
 lemma A_trusts_NS2:
-     "\\<lbrakk>Crypt (shrK A) \\<lbrace>NA, Agent B, Key K, X\\<rbrace> \\<in> parts (spies evs);
-       A \\<notin> bad;  evs \\<in> ns_shared\\<rbrakk>
-      \\<Longrightarrow> Says Server A (Crypt (shrK A) \\<lbrace>NA, Agent B, Key K, X\\<rbrace>) \\<in> set evs"
+     "\<lbrakk>Crypt (shrK A) \<lbrace>NA, Agent B, Key K, X\<rbrace> \<in> parts (spies evs);
+       A \<notin> bad;  evs \<in> ns_shared\<rbrakk>
+      \<Longrightarrow> Says Server A (Crypt (shrK A) \<lbrace>NA, Agent B, Key K, X\<rbrace>) \<in> set evs"
 apply (erule rev_mp)
 apply (erule ns_shared.induct, force, drule_tac [4] NS3_msg_in_parts_spies, auto)
 done
 
 lemma cert_A_form:
-     "\\<lbrakk>Crypt (shrK A) \\<lbrace>NA, Agent B, Key K, X\\<rbrace> \\<in> parts (spies evs);
-       A \\<notin> bad;  evs \\<in> ns_shared\\<rbrakk>
-      \\<Longrightarrow> K \\<notin> range shrK \\<and>  X = (Crypt (shrK B) \\<lbrace>Key K, Agent A\\<rbrace>)"
+     "\<lbrakk>Crypt (shrK A) \<lbrace>NA, Agent B, Key K, X\<rbrace> \<in> parts (spies evs);
+       A \<notin> bad;  evs \<in> ns_shared\<rbrakk>
+      \<Longrightarrow> K \<notin> range shrK \<and>  X = (Crypt (shrK B) \<lbrace>Key K, Agent A\<rbrace>)"
 by (blast dest!: A_trusts_NS2 Says_Server_message_form)
 
 (*EITHER describes the form of X when the following message is sent,
   OR     reduces it to the Fake case.
   Use Says_Server_message_form if applicable.*)
 lemma Says_S_message_form:
-     "\\<lbrakk>Says S A (Crypt (shrK A) \\<lbrace>Nonce NA, Agent B, Key K, X\\<rbrace>) \\<in> set evs;
-       evs \\<in> ns_shared\\<rbrakk>
-      \\<Longrightarrow> (K \\<notin> range shrK \\<and> X = (Crypt (shrK B) \\<lbrace>Key K, Agent A\\<rbrace>))
-          \\<or> X \\<in> analz (spies evs)"
+     "\<lbrakk>Says S A (Crypt (shrK A) \<lbrace>Nonce NA, Agent B, Key K, X\<rbrace>) \<in> set evs;
+       evs \<in> ns_shared\<rbrakk>
+      \<Longrightarrow> (K \<notin> range shrK \<and> X = (Crypt (shrK B) \<lbrace>Key K, Agent A\<rbrace>))
+          \<or> X \<in> analz (spies evs)"
 by (blast dest: Says_imp_knows_Spy cert_A_form analz.Inj)
 
 
 (*Alternative version also provable
 lemma Says_S_message_form2:
-  "\\<lbrakk>Says S A (Crypt (shrK A) \\<lbrace>Nonce NA, Agent B, Key K, X\\<rbrace>) \\<in> set evs;
-    evs \\<in> ns_shared\\<rbrakk>
-   \\<Longrightarrow> Says Server A (Crypt (shrK A) \\<lbrace>Nonce NA, Agent B, Key K, X\\<rbrace>) \\<in> set evs
-       \\<or> X \\<in> analz (spies evs)"
-apply (case_tac "A \\<in> bad")
+  "\<lbrakk>Says S A (Crypt (shrK A) \<lbrace>Nonce NA, Agent B, Key K, X\<rbrace>) \<in> set evs;
+    evs \<in> ns_shared\<rbrakk>
+   \<Longrightarrow> Says Server A (Crypt (shrK A) \<lbrace>Nonce NA, Agent B, Key K, X\<rbrace>) \<in> set evs
+       \<or> X \<in> analz (spies evs)"
+apply (case_tac "A \<in> bad")
 apply (force dest!: Says_imp_knows_Spy [THEN analz.Inj])
 by (blast dest!: A_trusts_NS2 Says_Server_message_form)
 *)
@@ -185,35 +185,35 @@ by (blast dest!: A_trusts_NS2 Says_Server_message_form)
 (****
  SESSION KEY COMPROMISE THEOREM.  To prove theorems of the form
 
-  Key K \\<in> analz (insert (Key KAB) (spies evs)) \\<Longrightarrow>
-  Key K \\<in> analz (spies evs)
+  Key K \<in> analz (insert (Key KAB) (spies evs)) \<Longrightarrow>
+  Key K \<in> analz (spies evs)
 
  A more general formula must be proved inductively.
 ****)
 
-(*NOT useful in this form, but it says that session keys are not used
+text{*NOT useful in this form, but it says that session keys are not used
   to encrypt messages containing other keys, in the actual protocol.
-  We require that agents should behave like this subsequently also.*)
-lemma  "\\<lbrakk>evs \\<in> ns_shared;  Kab \\<notin> range shrK\\<rbrakk> \\<Longrightarrow>
-         (Crypt KAB X) \\<in> parts (spies evs) \\<and>
-         Key K \\<in> parts {X} \\<longrightarrow> Key K \\<in> parts (spies evs)"
+  We require that agents should behave like this subsequently also.*}
+lemma  "\<lbrakk>evs \<in> ns_shared;  Kab \<notin> range shrK\<rbrakk> \<Longrightarrow>
+         (Crypt KAB X) \<in> parts (spies evs) \<and>
+         Key K \<in> parts {X} \<longrightarrow> Key K \<in> parts (spies evs)"
 apply (erule ns_shared.induct, force, drule_tac [4] NS3_msg_in_parts_spies, simp_all)
-(*Fake*)
+txt{*Fake*}
 apply (blast dest: parts_insert_subset_Un)
-(*Base, NS4 and NS5*)
+txt{*Base, NS4 and NS5*}
 apply auto
 done
 
 
-(** Session keys are not used to encrypt other session keys **)
+subsubsection{*Session keys are not used to encrypt other session keys*}
 
-(*The equality makes the induction hypothesis easier to apply*)
+text{*The equality makes the induction hypothesis easier to apply*}
 
 lemma analz_image_freshK [rule_format]:
- "evs \\<in> ns_shared \\<Longrightarrow>
-   \\<forall>K KK. KK \\<subseteq> - (range shrK) \\<longrightarrow>
-             (Key K \\<in> analz (Key`KK \\<union> (spies evs))) =
-             (K \\<in> KK \\<or> Key K \\<in> analz (spies evs))"
+ "evs \<in> ns_shared \<Longrightarrow>
+   \<forall>K KK. KK \<subseteq> - (range shrK) \<longrightarrow>
+             (Key K \<in> analz (Key`KK \<union> (spies evs))) =
+             (K \<in> KK \<or> Key K \<in> analz (spies evs))"
 apply (erule ns_shared.induct, force)
 apply (drule_tac [7] Says_Server_message_form)
 apply (erule_tac [4] Says_S_message_form [THEN disjE], analz_freshK, spy_analz)
@@ -221,97 +221,100 @@ done
 
 
 lemma analz_insert_freshK:
-     "\\<lbrakk>evs \\<in> ns_shared;  KAB \\<notin> range shrK\\<rbrakk> \\<Longrightarrow>
-       (Key K \\<in> analz (insert (Key KAB) (spies evs))) =
-       (K = KAB \\<or> Key K \\<in> analz (spies evs))"
+     "\<lbrakk>evs \<in> ns_shared;  KAB \<notin> range shrK\<rbrakk> \<Longrightarrow>
+       (Key K \<in> analz (insert (Key KAB) (spies evs))) =
+       (K = KAB \<or> Key K \<in> analz (spies evs))"
 by (simp only: analz_image_freshK analz_image_freshK_simps)
 
 
-(** The session key K uniquely identifies the message **)
+subsubsection{*The session key K uniquely identifies the message*}
 
-(*In messages of this form, the session key uniquely identifies the rest*)
+text{*In messages of this form, the session key uniquely identifies the rest*}
 lemma unique_session_keys:
-     "\\<lbrakk>Says Server A (Crypt (shrK A) \\<lbrace>NA, Agent B, Key K, X\\<rbrace>) \\<in> set evs;
-       Says Server A' (Crypt (shrK A') \\<lbrace>NA', Agent B', Key K, X'\\<rbrace>) \\<in> set evs;
-       evs \\<in> ns_shared\\<rbrakk> \\<Longrightarrow> A=A' \\<and> NA=NA' \\<and> B=B' \\<and> X = X'"
+     "\<lbrakk>Says Server A (Crypt (shrK A) \<lbrace>NA, Agent B, Key K, X\<rbrace>) \<in> set evs;
+       Says Server A' (Crypt (shrK A') \<lbrace>NA', Agent B', Key K, X'\<rbrace>) \<in> set evs;
+       evs \<in> ns_shared\<rbrakk> \<Longrightarrow> A=A' \<and> NA=NA' \<and> B=B' \<and> X = X'"
 apply (erule rev_mp, erule rev_mp, erule ns_shared.induct, simp_all, blast+)
 done
 
 
-(** Crucial secrecy property: Spy does not see the keys sent in msg NS2 **)
+subsubsection{*Crucial secrecy property: Spy does not see the keys sent in msg NS2*}
 
-(*Beware of [rule_format] and the universal quantifier!*)
+text{*Beware of [rule_format] and the universal quantifier!*}
 lemma secrecy_lemma:
-     "\\<lbrakk>Says Server A (Crypt (shrK A) \\<lbrace>NA, Agent B, Key K,
-                                      Crypt (shrK B) \\<lbrace>Key K, Agent A\\<rbrace>\\<rbrace>)
-              \\<in> set evs;
-         A \\<notin> bad;  B \\<notin> bad;  evs \\<in> ns_shared\\<rbrakk>
-      \\<Longrightarrow> (\\<forall>NB. Notes Spy \\<lbrace>NA, NB, Key K\\<rbrace> \\<notin> set evs) \\<longrightarrow>
-         Key K \\<notin> analz (spies evs)"
+     "\<lbrakk>Says Server A (Crypt (shrK A) \<lbrace>NA, Agent B, Key K,
+                                      Crypt (shrK B) \<lbrace>Key K, Agent A\<rbrace>\<rbrace>)
+              \<in> set evs;
+         A \<notin> bad;  B \<notin> bad;  evs \<in> ns_shared\<rbrakk>
+      \<Longrightarrow> (\<forall>NB. Notes Spy \<lbrace>NA, NB, Key K\<rbrace> \<notin> set evs) \<longrightarrow>
+         Key K \<notin> analz (spies evs)"
 apply (erule rev_mp)
 apply (erule ns_shared.induct, force)
 apply (frule_tac [7] Says_Server_message_form)
 apply (frule_tac [4] Says_S_message_form)
 apply (erule_tac [5] disjE)
-apply (simp_all add: analz_insert_eq analz_insert_freshK pushes split_ifs, spy_analz)  (*Fake*)
-apply blast      (*NS2*)
-(*NS3, Server sub-case*) (**LEVEL 8 **)
+apply (simp_all add: analz_insert_eq analz_insert_freshK pushes split_ifs, spy_analz)  
+txt{*NS2*}
+apply blast
+txt{*NS3, Server sub-case*} 
 apply (blast dest!: Crypt_Spy_analz_bad A_trusts_NS2
 	     dest:  Says_imp_knows_Spy analz.Inj unique_session_keys)
-(*NS3, Spy sub-case; also Oops*)
+txt{*NS3, Spy sub-case; also Oops*}
 apply (blast dest: unique_session_keys)+
 done
 
 
 
-(*Final version: Server's message in the most abstract form*)
+text{*Final version: Server's message in the most abstract form*}
 lemma Spy_not_see_encrypted_key:
-     "\\<lbrakk>Says Server A (Crypt K' \\<lbrace>NA, Agent B, Key K, X\\<rbrace>) \\<in> set evs;
-       \\<forall>NB. Notes Spy \\<lbrace>NA, NB, Key K\\<rbrace> \\<notin> set evs;
-       A \\<notin> bad;  B \\<notin> bad;  evs \\<in> ns_shared\\<rbrakk>
-      \\<Longrightarrow> Key K \\<notin> analz (spies evs)"
+     "\<lbrakk>Says Server A (Crypt K' \<lbrace>NA, Agent B, Key K, X\<rbrace>) \<in> set evs;
+       \<forall>NB. Notes Spy \<lbrace>NA, NB, Key K\<rbrace> \<notin> set evs;
+       A \<notin> bad;  B \<notin> bad;  evs \<in> ns_shared\<rbrakk>
+      \<Longrightarrow> Key K \<notin> analz (spies evs)"
 by (blast dest: Says_Server_message_form secrecy_lemma)
 
 
-(**** Guarantees available at various stages of protocol ***)
+subsection{*Guarantees available at various stages of protocol*}
 
-(*If the encrypted message appears then it originated with the Server*)
+text{*If the encrypted message appears then it originated with the Server*}
 lemma B_trusts_NS3:
-     "\\<lbrakk>Crypt (shrK B) \\<lbrace>Key K, Agent A\\<rbrace> \\<in> parts (spies evs);
-       B \\<notin> bad;  evs \\<in> ns_shared\\<rbrakk>
-      \\<Longrightarrow> \\<exists>NA. Says Server A
-               (Crypt (shrK A) \\<lbrace>NA, Agent B, Key K,
-                                 Crypt (shrK B) \\<lbrace>Key K, Agent A\\<rbrace>\\<rbrace>)
-              \\<in> set evs"
+     "\<lbrakk>Crypt (shrK B) \<lbrace>Key K, Agent A\<rbrace> \<in> parts (spies evs);
+       B \<notin> bad;  evs \<in> ns_shared\<rbrakk>
+      \<Longrightarrow> \<exists>NA. Says Server A
+               (Crypt (shrK A) \<lbrace>NA, Agent B, Key K,
+                                 Crypt (shrK B) \<lbrace>Key K, Agent A\<rbrace>\<rbrace>)
+              \<in> set evs"
 apply (erule rev_mp)
 apply (erule ns_shared.induct, force, drule_tac [4] NS3_msg_in_parts_spies, auto)
 done
 
 
 lemma A_trusts_NS4_lemma [rule_format]:
-   "evs \\<in> ns_shared \\<Longrightarrow>
-      Key K \\<notin> analz (spies evs) \\<longrightarrow>
-      Says Server A (Crypt (shrK A) \\<lbrace>NA, Agent B, Key K, X\\<rbrace>) \\<in> set evs \\<longrightarrow>
-      Crypt K (Nonce NB) \\<in> parts (spies evs) \\<longrightarrow>
-      Says B A (Crypt K (Nonce NB)) \\<in> set evs"
+   "evs \<in> ns_shared \<Longrightarrow>
+      Key K \<notin> analz (spies evs) \<longrightarrow>
+      Says Server A (Crypt (shrK A) \<lbrace>NA, Agent B, Key K, X\<rbrace>) \<in> set evs \<longrightarrow>
+      Crypt K (Nonce NB) \<in> parts (spies evs) \<longrightarrow>
+      Says B A (Crypt K (Nonce NB)) \<in> set evs"
 apply (erule ns_shared.induct, force, drule_tac [4] NS3_msg_in_parts_spies)
-apply (analz_mono_contra, simp_all, blast)     (*Fake*)
+apply (analz_mono_contra, simp_all, blast) 
 (*NS2: contradiction from the assumptions
-  Key K \\<notin> used evs2  and Crypt K (Nonce NB) \\<in> parts (spies evs2) *)
-apply (force dest!: Crypt_imp_keysFor, blast)     (*NS3*)
-(*NS4*)
+  Key K \<notin> used evs2  and Crypt K (Nonce NB) \<in> parts (spies evs2) *)
+apply (force dest!: Crypt_imp_keysFor)     
+txt{*NS3*}
+apply blast 
+txt{*NS4*}
 apply (blast dest!: B_trusts_NS3
 	     dest: Says_imp_knows_Spy [THEN analz.Inj]
                    Crypt_Spy_analz_bad unique_session_keys)
 done
 
-(*This version no longer assumes that K is secure*)
+text{*This version no longer assumes that K is secure*}
 lemma A_trusts_NS4:
-     "\\<lbrakk>Crypt K (Nonce NB) \\<in> parts (spies evs);
-       Crypt (shrK A) \\<lbrace>NA, Agent B, Key K, X\\<rbrace> \\<in> parts (spies evs);
-       \\<forall>NB. Notes Spy \\<lbrace>NA, NB, Key K\\<rbrace> \\<notin> set evs;
-       A \\<notin> bad;  B \\<notin> bad;  evs \\<in> ns_shared\\<rbrakk>
-      \\<Longrightarrow> Says B A (Crypt K (Nonce NB)) \\<in> set evs"
+     "\<lbrakk>Crypt K (Nonce NB) \<in> parts (spies evs);
+       Crypt (shrK A) \<lbrace>NA, Agent B, Key K, X\<rbrace> \<in> parts (spies evs);
+       \<forall>NB. Notes Spy \<lbrace>NA, NB, Key K\<rbrace> \<notin> set evs;
+       A \<notin> bad;  B \<notin> bad;  evs \<in> ns_shared\<rbrakk>
+      \<Longrightarrow> Says B A (Crypt K (Nonce NB)) \<in> set evs"
 by (blast intro: A_trusts_NS4_lemma
           dest: A_trusts_NS2 Spy_not_see_encrypted_key)
 
@@ -319,16 +322,18 @@ by (blast intro: A_trusts_NS4_lemma
   component X in some instance of NS4.  Perhaps an interesting property,
   but not needed (after all) for the proofs below.*)
 theorem NS4_implies_NS3 [rule_format]:
-  "evs \\<in> ns_shared \\<Longrightarrow>
-     Key K \\<notin> analz (spies evs) \\<longrightarrow>
-     Says Server A (Crypt (shrK A) \\<lbrace>NA, Agent B, Key K, X\\<rbrace>) \\<in> set evs \\<longrightarrow>
-     Crypt K (Nonce NB) \\<in> parts (spies evs) \\<longrightarrow>
-     (\\<exists>A'. Says A' B X \\<in> set evs)"
+  "evs \<in> ns_shared \<Longrightarrow>
+     Key K \<notin> analz (spies evs) \<longrightarrow>
+     Says Server A (Crypt (shrK A) \<lbrace>NA, Agent B, Key K, X\<rbrace>) \<in> set evs \<longrightarrow>
+     Crypt K (Nonce NB) \<in> parts (spies evs) \<longrightarrow>
+     (\<exists>A'. Says A' B X \<in> set evs)"
 apply (erule ns_shared.induct, force, drule_tac [4] NS3_msg_in_parts_spies, analz_mono_contra)
-apply (simp_all add: ex_disj_distrib, blast)  (*Fake*)
-apply (blast dest!: new_keys_not_used Crypt_imp_keysFor)  (*NS2*)
-apply blast  (*NS3*)
-(*NS4*)
+apply (simp_all add: ex_disj_distrib, blast)
+txt{*NS2*}
+apply (blast dest!: new_keys_not_used Crypt_imp_keysFor)  
+txt{*NS3*}
+apply blast
+txt{*NS4*}
 apply (blast dest!: B_trusts_NS3
 	     dest: Says_imp_knows_Spy [THEN analz.Inj]
                    unique_session_keys Crypt_Spy_analz_bad)
@@ -336,30 +341,32 @@ done
 
 
 lemma B_trusts_NS5_lemma [rule_format]:
-  "\\<lbrakk>B \\<notin> bad;  evs \\<in> ns_shared\\<rbrakk> \\<Longrightarrow>
-     Key K \\<notin> analz (spies evs) \\<longrightarrow>
+  "\<lbrakk>B \<notin> bad;  evs \<in> ns_shared\<rbrakk> \<Longrightarrow>
+     Key K \<notin> analz (spies evs) \<longrightarrow>
      Says Server A
-	  (Crypt (shrK A) \\<lbrace>NA, Agent B, Key K,
-			    Crypt (shrK B) \\<lbrace>Key K, Agent A\\<rbrace>\\<rbrace>) \\<in> set evs \\<longrightarrow>
-     Crypt K \\<lbrace>Nonce NB, Nonce NB\\<rbrace> \\<in> parts (spies evs) \\<longrightarrow>
-     Says A B (Crypt K \\<lbrace>Nonce NB, Nonce NB\\<rbrace>) \\<in> set evs"
-apply (erule ns_shared.induct, force, drule_tac [4] NS3_msg_in_parts_spies, analz_mono_contra, simp_all, blast)  (*Fake*)
-apply (blast dest!: new_keys_not_used Crypt_imp_keysFor)  (*NS2*)
-apply (blast dest!: cert_A_form) (*NS3*)
-(*NS5*)
+	  (Crypt (shrK A) \<lbrace>NA, Agent B, Key K,
+			    Crypt (shrK B) \<lbrace>Key K, Agent A\<rbrace>\<rbrace>) \<in> set evs \<longrightarrow>
+     Crypt K \<lbrace>Nonce NB, Nonce NB\<rbrace> \<in> parts (spies evs) \<longrightarrow>
+     Says A B (Crypt K \<lbrace>Nonce NB, Nonce NB\<rbrace>) \<in> set evs"
+apply (erule ns_shared.induct, force, drule_tac [4] NS3_msg_in_parts_spies, analz_mono_contra, simp_all, blast)
+txt{*NS2*}
+apply (blast dest!: new_keys_not_used Crypt_imp_keysFor)  
+txt{*NS3*}
+apply (blast dest!: cert_A_form) 
+txt{*NS5*}
 apply (blast dest!: A_trusts_NS2
 	     dest: Says_imp_knows_Spy [THEN analz.Inj]
                    unique_session_keys Crypt_Spy_analz_bad)
 done
 
 
-(*Very strong Oops condition reveals protocol's weakness*)
+text{*Very strong Oops condition reveals protocol's weakness*}
 lemma B_trusts_NS5:
-     "\\<lbrakk>Crypt K \\<lbrace>Nonce NB, Nonce NB\\<rbrace> \\<in> parts (spies evs);
-       Crypt (shrK B) \\<lbrace>Key K, Agent A\\<rbrace> \\<in> parts (spies evs);
-       \\<forall>NA NB. Notes Spy \\<lbrace>NA, NB, Key K\\<rbrace> \\<notin> set evs;
-       A \\<notin> bad;  B \\<notin> bad;  evs \\<in> ns_shared\\<rbrakk>
-      \\<Longrightarrow> Says A B (Crypt K \\<lbrace>Nonce NB, Nonce NB\\<rbrace>) \\<in> set evs"
+     "\<lbrakk>Crypt K \<lbrace>Nonce NB, Nonce NB\<rbrace> \<in> parts (spies evs);
+       Crypt (shrK B) \<lbrace>Key K, Agent A\<rbrace> \<in> parts (spies evs);
+       \<forall>NA NB. Notes Spy \<lbrace>NA, NB, Key K\<rbrace> \<notin> set evs;
+       A \<notin> bad;  B \<notin> bad;  evs \<in> ns_shared\<rbrakk>
+      \<Longrightarrow> Says A B (Crypt K \<lbrace>Nonce NB, Nonce NB\<rbrace>) \<in> set evs"
 by (blast intro: B_trusts_NS5_lemma
           dest: B_trusts_NS3 Spy_not_see_encrypted_key)
 
